src/Disks/ZonedDisk.dfy
@@ -6,6 +6,9 @@ module Zone {
     import opened NativeTypes
     import Block
 
+    // XXX: should Constants be the zone size, and
+    // then the ZonedDisk zonemap be a seq of Zone.Constants?
+
     datatype State = State(
         write_ptr: uint64,
         blocks: seq<Block.State>
@@ -47,26 +50,29 @@ module Zone {
         && s'.blocks[s.write_ptr] == b
     }
 
-    predicate Reset(s: State)
+    function method Reset(s: State) : State
         requires Valid(s)
+        ensures Valid(Reset(s))
     {
-        s.write_ptr == 0
+        var blocks := |s.blocks|;
+
+        State(
+            write_ptr := 0,
+            blocks := seq(blocks, i => Block.Init()))
     }
 
     predicate Empty(s: State)
-        requires Valid(s)
     {
         s.write_ptr == 0
     }
 
     predicate Full(s: State)
-        requires Valid(s)
     {
         s.write_ptr as int == |s.blocks|
     }
 }
 
-module ZonedDisk /* refines Disk */ {
+module ZonedDisk refines Disk {
     import opened NativeTypes
     import opened Types
     import opened Zone
@@ -81,12 +87,42 @@ module ZonedDisk /* refines Disk */ {
     )
 
     function method Init(c: Constants) : State
-        requires ConstantsValid(c)
     {
         State.State(
             seq(|c.zone_map|, i => Zone.Init(c.zone_map[i].1 - c.zone_map[i].0))
         )
     }
+
+    function method Read(c: Constants, s: State, zone: uint64, block: uint64) : Block.State
+        requires Valid(c, s)
+        ensures Block.Valid(Read(c, s, zone, block))
+    {
+        s.zones[zone].blocks[block]
+    }
+
+    predicate Append(c: Constants, s: State, s': State, zone_id: uint64, block: Block.State)
+        requires Valid(c, s)
+        ensures Valid(c, s')
+    {
+        var write_ptr := s.zones[zone_id].write_ptr;
+        var pre_blocks := s.zones[zone_id].blocks[write_ptr := block];
+        var post_blocks := s'.zones[zone_id].blocks[0..write_ptr + 1];
+
+        && 0 <= zone_id < |c.zone_map| as uint64
+        && s'.zones[zone_id].write_ptr == write_ptr + 1
+        && pre_blocks[0..write_ptr + 1] == post_blocks
+    }
+
+    predicate Reset(c: Constants, s: State, s': State, zone_id: uint64)
+        requires Valid(c, s)
+    {
+        && forall i :: 0 <= i < |c.zone_map| 
+            ==> i != zone_id as int 
+            ==> s.zones[i] == s'.zones[i]
+        && s'.zones[zone_id] == Zone.Reset(s.zones[zone_id])
+    }
+
+    // Invariants
 
     predicate ConstantsValid(c: Constants)
     {
@@ -97,6 +133,8 @@ module ZonedDisk /* refines Disk */ {
     {
         && ConstantsValid(c)
         && |s.zones| == |c.zone_map|
+        && forall i :: 0 <= i < |c.zone_map|
+            ==> |s.zones[i].blocks| == (c.zone_map[i].1 - c.zone_map[i].0) as int
     }
 
 
@@ -143,7 +181,46 @@ module ZonedDisk /* refines Disk */ {
         }
     }
 
+    // Steps and step relations
+
     datatype Step =
-    | ReadBlock(block: uint32, contents: seq<uint8>)
-    | WriteBlock(tid: uint32, contents: seq<uint8>)
+    | ReadFromZone(zone: uint64, block: uint64, val: Block.State)
+    | AppendToZone(zone_idx: uint64, contents: seq<uint8>)
+    | ResetZone(zone_idx: uint64)
+
+    predicate NextStep(c: Constants, s: State, s': State, step: Step)
+    {
+        Valid(c, s) && match step
+        {
+            case ReadFromZone(zone, block, val) =>
+                && 0 <= zone as int < |s.zones|
+                && Read(c, s, zone, block) == val
+                && s == s'
+
+            case AppendToZone(zone, val) => 
+                && 0 <= zone as int < |s.zones| == |s'.zones|
+                && Append(c, s, s', zone, val)
+
+            case ResetZone(zone) => 
+                && 0 <= zone as int < |s.zones|
+                && Reset(c, s, s', zone)
+        }
+    }
+
+    predicate Next(c: Constants, s: State, s': State)
+    {
+        exists step :: NextStep(c, s, s', step)
+    }
+
+    // Invariant preservation
+
+    lemma InitImpliesValid(c: Constants)
+        {}
+
+    lemma NextPreservesValid(c: Constants, s: State, s': State)
+        requires Valid(c, s)
+        requires Next(c, s, s')
+        ensures Valid(c, s')
+    {
+    }
 }
